Start working on reloctablesgenproof

x86/Reloctablesgenproof.v
@@ -8,6 +8,7 @@ Require Import Integers Floats AST Linking.
 Require Import Values Memory Events Globalenvs Smallstep.
 Require Import Op Locations Mach Conventions Asm RealAsm.
 Require Import RelocProgram RelocProgSemantics RelocProgSemantics1.
+Require Import Symbtablegen.
 Require Import Reloctablesgen.
 Import ListNotations.
 
@@ -31,6 +32,1300 @@ Variables prog tprog: RelocProgram.program.
 
 Hypothesis TRANSF: match_prog prog tprog.
 
+Let ge := RelocProgSemantics.globalenv prog.
+Let tge := globalenv tprog.
+
+(* (* Given relocentry [e] and symtable [stbl], updates the mapping [m] that *)
+(* associates relocation offsets with their identifiers. *) *)
+(* Definition acc_reloc_ofs_symb (stbl:symbtable) (e:relocentry) (m:ZTree.t ident) : ZTree.t ident := *)
+(*   match SeqTable.get (reloc_symb e) stbl with *)
+(*   | None => m *)
+(*   | Some s => *)
+(*     match symbentry_id s with *)
+(*     | None => m *)
+(*     | Some id => ZTree.set (reloc_offset e) id m *)
+(*     end *)
+(*   end. *)
+
+(* Definition gen_reloc_ofs_symb (stbl: symbtable) (rtbl: reloctable) : ZTree.t ident := *)
+(*   fold_right (acc_reloc_ofs_symb stbl) (ZTree.empty ident) rtbl. *)
+
+Lemma acc_reloc_ofs_symb_ok:
+  forall stbl e m s id,
+    SeqTable.SeqTable.get (reloc_symb e) stbl = Some s ->
+    symbentry_id s = Some id ->
+    Maps.ZTree.get (reloc_offset e) (acc_reloc_ofs_symb stbl e m) = Some id.
+Proof.
+  unfold acc_reloc_ofs_symb. intros stbl e m s id STBL ID.
+  rewrite STBL, ID. rewrite Maps.ZTree.gss. auto.
+Qed.
+
+Lemma acc_reloc_ofs_symb_other:
+  forall stbl e m o,
+    o <> reloc_offset e ->
+    Maps.ZTree.get o (acc_reloc_ofs_symb stbl e m) = Maps.ZTree.get o m.
+Proof.
+  unfold acc_reloc_ofs_symb. intros stbl e m o DIFF.
+  destr. destr. rewrite Maps.ZTree.gso. auto. auto.
+Qed.
+
+Lemma gen_reloc_ofs_symb_ok:
+  forall stbl rtbl e s id,
+    In e rtbl ->
+    list_norepet (map (fun e => reloc_offset e) rtbl) ->
+    SeqTable.SeqTable.get (reloc_symb e) stbl = Some s ->
+    symbentry_id s = Some id ->
+    Maps.ZTree.get (reloc_offset e) (gen_reloc_ofs_symb stbl rtbl) = Some id.
+Proof.
+  induction rtbl; simpl. easy.
+  intros e s id [EQ|IN] NR STBL ID.
+  - subst.
+    eapply acc_reloc_ofs_symb_ok; eauto.
+  - rewrite acc_reloc_ofs_symb_other.
+    eapply IHrtbl; eauto. inv NR; auto.
+    inv NR. intro EQ.
+    apply H1.
+    rewrite in_map_iff. exists e; split; eauto.
+Qed.
+
+Lemma gen_reloc_ofs_symb_other:
+  forall stbl rtbl o,
+    ~ In o (map reloc_offset rtbl) ->
+    Maps.ZTree.get o (gen_reloc_ofs_symb stbl rtbl) = None.
+Proof.
+  induction rtbl; simpl. intros. rewrite Maps.ZTree.gempty. auto.
+  intros o NIN.
+  rewrite acc_reloc_ofs_symb_other. 2: intuition.
+  apply IHrtbl. intuition.
+Qed.
+
+(* Definition add_reloc_ofs_symb (stbl: symbtable) (i:reloctable_id)  (rmap: reloctable_map) *)
+(*            (ofsmap: reloctable_id -> ZTree.t ident) := *)
+(*   let rtbl := get_reloctable i rmap in *)
+(*   let m := gen_reloc_ofs_symb stbl rtbl in *)
+(*   fun i' => if reloctable_id_eq i i' then m else ofsmap i'. *)
+
+Lemma add_reloc_ofs_symb_diff_rtbl_id:
+  forall stbl rtbl_id rtbl_id' rmap ofsmap o,
+    rtbl_id <> rtbl_id' ->
+    Maps.ZTree.get o ((add_reloc_ofs_symb stbl rtbl_id rmap ofsmap) rtbl_id') =
+    Maps.ZTree.get o (ofsmap rtbl_id').
+Proof.
+  intros. unfold add_reloc_ofs_symb. destr.
+Qed.
+
+Lemma add_reloc_ofs_symb_same_rtbl_id_in:
+  forall stbl rtbl_id rmap ofsmap e s id,
+    let rtbl := get_reloctable rtbl_id rmap in
+    In e rtbl ->
+    list_norepet (map (fun e => reloc_offset e) rtbl) ->
+    SeqTable.SeqTable.get (reloc_symb e) stbl = Some s ->
+    symbentry_id s = Some id ->
+    Maps.ZTree.get (reloc_offset e) ((add_reloc_ofs_symb stbl rtbl_id rmap ofsmap) rtbl_id) = Some id.
+Proof.
+  intros. unfold add_reloc_ofs_symb. destr.
+  eapply gen_reloc_ofs_symb_ok; eauto.
+Qed.
+
+Lemma add_reloc_ofs_symb_same_rtbl_id_not_in:
+  forall stbl rtbl_id rmap ofsmap o,
+    let rtbl := get_reloctable rtbl_id rmap in
+    ~ In o (map reloc_offset rtbl) ->
+    Maps.ZTree.get o ((add_reloc_ofs_symb stbl rtbl_id rmap ofsmap) rtbl_id) =
+    None.
+Proof.
+  intros. unfold add_reloc_ofs_symb. destr.
+  eapply gen_reloc_ofs_symb_other; eauto.
+Qed.
+
+(* Definition gen_reloc_ofs_symbs (p:program) := *)
+(*   let stbl := p.(prog_symbtable) in *)
+(*   let rmap := p.(prog_reloctables) in *)
+(*   let ofsmap := fun i => ZTree.empty ident in *)
+(*   let ofsmap1 := add_reloc_ofs_symb stbl RELOC_DATA rmap ofsmap in *)
+(*   let ofsmap2 := add_reloc_ofs_symb stbl RELOC_CODE rmap ofsmap1 in *)
+(*   ofsmap2. *)
+
+Lemma gen_reloc_ofs_symbs_ok:
+  forall p rtbl_id e s id,
+    let rtbl := get_reloctable rtbl_id (prog_reloctables p) in
+    In e rtbl ->
+    list_norepet (map reloc_offset rtbl) ->
+    SeqTable.SeqTable.get (reloc_symb e) (prog_symbtable p) = Some s ->
+    symbentry_id s = Some id ->
+    Maps.ZTree.get (reloc_offset e) (gen_reloc_ofs_symbs p rtbl_id) = Some id.
+Proof.
+  intros. unfold gen_reloc_ofs_symbs.
+  destruct rtbl_id.
+  - eapply add_reloc_ofs_symb_same_rtbl_id_in; eauto.
+  - rewrite add_reloc_ofs_symb_diff_rtbl_id; eauto. 2: congruence.
+    eapply add_reloc_ofs_symb_same_rtbl_id_in; eauto.
+Qed.
+
+Lemma gen_reloc_ofs_symbs_not_in:
+  forall p rtbl_id o,
+    let rtbl := get_reloctable rtbl_id (prog_reloctables p) in
+    ~ In o (map reloc_offset rtbl) ->
+    Maps.ZTree.get o (gen_reloc_ofs_symbs p rtbl_id) = None.
+Proof.
+  intros. unfold gen_reloc_ofs_symbs.
+  destruct rtbl_id.
+  - eapply add_reloc_ofs_symb_same_rtbl_id_not_in; eauto.
+  - rewrite add_reloc_ofs_symb_diff_rtbl_id; eauto. 2: congruence.
+    eapply add_reloc_ofs_symb_same_rtbl_id_not_in; eauto.
+Qed.
+
+(* Definition globalenv (p: program) : Genv.t := *)
+(*   let ofsmap := gen_reloc_ofs_symbs p in *)
+(*   let genv1 := RelocProgSemantics.globalenv p in *)
+(*   Genv.mkgenv ofsmap genv1. *)
+
+
+Lemma genv_reloc_ofs_symb_ok:
+  forall p rtbl_id e s id,
+    let rtbl := get_reloctable rtbl_id (prog_reloctables p) in
+    In e rtbl ->
+    list_norepet (map reloc_offset rtbl) ->
+    SeqTable.SeqTable.get (reloc_symb e) (prog_symbtable p) = Some s ->
+    symbentry_id s = Some id ->
+    Maps.ZTree.get (reloc_offset e) (Genv.genv_reloc_ofs_symb (globalenv p) rtbl_id) = Some id.
+Proof.
+  intros. unfold globalenv. simpl.
+  eapply gen_reloc_ofs_symbs_ok; eauto.
+Qed.
+
+Lemma genv_reloc_ofs_symb_not_in:
+  forall p rtbl_id o,
+    let rtbl := get_reloctable rtbl_id (prog_reloctables p) in
+    ~ In o (map reloc_offset rtbl) ->
+    Maps.ZTree.get o (Genv.genv_reloc_ofs_symb (globalenv p) rtbl_id) = None.
+Proof.
+  intros. unfold globalenv; simpl.
+  eapply gen_reloc_ofs_symbs_not_in; eauto.
+Qed.
+
+Lemma transl_sectable_ok:
+  forall sim stbl creloc dreloc,
+    transl_sectable sim stbl = OK (creloc, dreloc) ->
+    exists c l,
+      SeqTable.SeqTable.get sec_code_id stbl = Some (sec_text c) /\
+      SeqTable.SeqTable.get sec_data_id stbl = Some (sec_data l) /\
+      transl_code sim c = OK creloc /\
+      transl_init_data_list sim l = OK dreloc.
+Proof.
+  unfold transl_sectable. intros sim stbl creloc dreloc TRANSL.
+  repeat destr_in TRANSL. do 2 eexists; eauto.
+Qed.
+
+Lemma transl_init_data_ok:
+  forall sim dofs id ofs dreloc,
+    transl_init_data sim dofs (Init_addrof id ofs) = OK dreloc ->
+    exists idx,
+      Maps.PTree.get id sim = Some idx /\
+      dreloc = [ {| reloc_offset := dofs; reloc_type := reloc_abs; reloc_symb := idx; reloc_addend := Ptrofs.unsigned ofs |}].
+Proof.
+  unfold transl_init_data.
+  intros sim dofs id ofs dreloc TID.
+  destr_in TID. inv TID.
+  eexists; split; eauto.
+Qed.
+
+Lemma transl_init_data_nil:
+  forall sim dofs d,
+    (forall id ofs, d <> Init_addrof id ofs) ->
+    transl_init_data sim dofs d = OK [].
+Proof.
+  unfold transl_init_data.
+  intros sim dofs d NO. destr.
+Qed.
+
+Lemma acc_init_data_ok:
+  forall sim ofs l d ofs' l',
+    acc_init_data sim (OK (ofs, l)) d = OK (ofs', l') ->
+    exists d',
+      transl_init_data sim ofs d = OK d' /\
+      ofs' = ofs + init_data_size d /\ l' = d' ++ l.
+Proof.
+  intros sim ofs l d ofs' l' AID.
+  unfold acc_init_data in AID.
+  monadInv AID. destr_in EQ0.
+  monadInv EQ0. inv EQ. eauto.
+Qed.
+
+Lemma transl_init_data_translate:
+  forall sim ofs d,
+    transl_init_data sim ofs d =
+    bind (transl_init_data sim 0 d) (fun rtbl =>
+                                       OK (map (fun d => {|
+                                                reloc_offset := reloc_offset d + ofs;
+                                                reloc_type := reloc_type d;
+                                                reloc_symb := reloc_symb d;
+                                                reloc_addend := reloc_addend d
+                                              |}) rtbl)).
+Proof.
+  intros sim ofs d.
+  unfold transl_init_data.
+  destr. destr.
+Qed.
+
+Lemma fold_acc_init_data_error:
+  forall sim l e,
+    fold_left (acc_init_data sim) l (Error e) = Error e.
+Proof.
+  induction l ; simpl; intros; eauto.
+Qed.
+
+Lemma fold_acc_init_data_ok:
+  forall sim l ofs rtbl,
+  fold_left (acc_init_data sim) l (OK (ofs, rtbl)) =
+  bind (fold_left (acc_init_data sim) l (OK (0, [])))
+       (fun '(ofs', rtbl') =>
+          OK (ofs + ofs', map (fun d => {|
+                                   reloc_offset := reloc_offset d + ofs;
+                                   reloc_type := reloc_type d;
+                                   reloc_symb := reloc_symb d;
+                                   reloc_addend := reloc_addend d
+                                 |}) rtbl' ++ rtbl)).
+Proof.
+  induction l; simpl; intros; eauto. repeat f_equal. omega.
+  rewrite transl_init_data_translate.
+  destruct (transl_init_data sim 0 a) eqn:?; simpl; auto.
+  - rewrite (IHl (ofs + init_data_size a)).
+    rewrite (IHl (init_data_size a)).
+    destruct (fold_left (acc_init_data sim) l (OK (0, []))); simpl; auto.
+    destr. simpl.
+    f_equal. f_equal. omega. simpl.
+    simpl.
+    rewrite ! app_assoc.
+    f_equal. rewrite app_nil_r.
+    rewrite list_append_map. f_equal.
+    rewrite map_map. simpl.
+    apply list_map_exten. intros. f_equal. omega.
+  - rewrite fold_acc_init_data_error. simpl. reflexivity.
+Qed.
+
+Lemma fold_acc_init_data_not_in:
+  forall sim l ofs rtbl ofs' rtbl',
+    fold_left (acc_init_data sim) l (OK (ofs, rtbl)) = OK (ofs', rtbl') ->
+    forall x, In x rtbl -> In x rtbl'.
+Proof.
+  induction l; simpl; intros; eauto.
+  inv H. auto.
+  destruct (transl_init_data sim ofs a); simpl in *.
+  eapply IHl. eauto. rewrite in_app. auto.
+  rewrite fold_acc_init_data_error in H; easy.
+Qed.
+
+Lemma transl_init_data_list_ok:
+  forall sim l dreloc l1 id o l2 symb_idx,
+    transl_init_data_list sim l = OK dreloc ->
+    l = l1 ++ Init_addrof id o :: l2 ->
+    Maps.PTree.get id sim = Some symb_idx ->
+    exists e ofs rtbl',
+      In e dreloc /\
+      fold_left (acc_init_data sim) l1 (OK (0, [])) = OK (ofs, rtbl') /\
+      reloc_offset e = ofs /\
+      reloc_type e = reloc_abs /\
+      reloc_symb e = symb_idx /\
+      reloc_addend e = Ptrofs.unsigned o.
+Proof.
+  intros sim l dreloc l1 id o l2 symb_idx TIDL SPLIT SYMB.
+  unfold transl_init_data_list in TIDL.
+  subst.
+  rewrite fold_left_app in TIDL.
+  monadInv TIDL.
+  destruct (fold_left (acc_init_data sim) l1 (OK (0, []))) eqn:?.
+  2: rewrite fold_acc_init_data_error in EQ; simpl in EQ; easy.
+  destr_in EQ0. inv EQ0.
+  simpl in EQ. destr_in EQ.
+  rewrite SYMB in EQ. simpl in EQ.
+  do 3 eexists. split. eapply fold_acc_init_data_not_in. apply EQ. left. reflexivity. simpl.
+  split. eauto. auto.
+Qed.
+
+
+Lemma symb_address_ok:
+  forall i b o ofs,
+  RelocProgSemantics.Genv.find_symbol ge i = Some (b, o) ->
+  RelocProgSemantics.Genv.symbol_address ge i ofs = Vptr b (Ptrofs.add ofs o).
+Proof.
+  intros.
+  unfold RelocProgSemantics.Genv.symbol_address. rewrite H. auto.
+Qed.
+
+Lemma add_external_global_symb_unchanged:
+  forall t e ge tge,
+    Genv.genv_symb ge = Genv.genv_symb tge ->
+    Genv.genv_next ge = Genv.genv_next tge ->
+    Genv.genv_symb (add_external_global t ge e) =
+    Genv.genv_symb (add_external_global t tge e) /\
+    Genv.genv_next (add_external_global t ge e) =
+    Genv.genv_next (add_external_global t tge e).
+Proof.
+  unfold add_external_global.
+  intros. destr. simpl. destr.
+Qed.
+
+Lemma add_external_globals_symb_unchanged:
+  forall t stbl ge tge,
+    Genv.genv_symb ge = Genv.genv_symb tge ->
+    Genv.genv_next ge = Genv.genv_next tge ->
+    Genv.genv_symb (add_external_globals t ge stbl) =
+    Genv.genv_symb (add_external_globals t tge stbl) /\
+    Genv.genv_next (add_external_globals t ge stbl) =
+    Genv.genv_next (add_external_globals t tge stbl)
+.
+Proof.
+  induction stbl; simpl; intros; eauto.
+  apply IHstbl.
+  apply add_external_global_symb_unchanged; auto.
+  apply add_external_global_symb_unchanged; auto.
+Qed.
+
+Lemma genv_symb_ok:
+  Genv.genv_symb (RelocProgSemantics.globalenv prog) =
+  Genv.genv_symb (RelocProgSemantics.globalenv tprog).
+Proof.
+  unfold match_prog in TRANSF.
+  unfold transf_program in TRANSF.
+  monadInv TRANSF.
+  unfold RelocProgSemantics.globalenv. simpl.
+  apply add_external_globals_symb_unchanged. simpl. auto. simpl. auto.
+Qed.
+
+Lemma symb_address_2:
+  forall e i
+         idx idofs b o s,
+    let rtbl := reloctable_data (prog_reloctables tprog) in
+    In e rtbl ->
+    list_norepet reloc_offset ## rtbl ->
+    SeqTable.SeqTable.get idx (prog_symbtable tprog) = Some s ->
+    symbentry_id s = Some i ->
+    (* Maps.PTree.get i sim = Some idx -> *)
+    reloc_symb e = idx ->
+    reloc_offset e = idofs ->
+    RelocProgSemantics.Genv.find_symbol ge i = Some (b, o) ->
+    Genv.find_symbol tge RELOC_DATA idofs = Some (b, o).
+Proof.
+  unfold Genv.find_symbol.
+  intros.
+  subst. unfold tge. erewrite genv_reloc_ofs_symb_ok. all: eauto.
+  unfold globalenv. simpl.
+  revert H5.
+  unfold RelocProgSemantics.Genv.find_symbol.
+  unfold ge.
+  rewrite genv_symb_ok. auto.
+Qed.
+
+
+Axiom nr_defs:
+  list_norepet (map fst (prog_defs tprog)).
+
+Axiom symb_table_ok:
+  forall id d,
+    In (id, d) (prog_defs tprog) ->
+    exists dofs1 cofs1,
+      In (Symbtablegen.get_symbentry sec_data_id sec_code_id dofs1 cofs1 id d) (prog_symbtable tprog).
+
+Lemma genv_symb_add_external_global:
+  forall t ge se id b o,
+    Maps.PTree.get id (Genv.genv_symb (add_external_global t ge se)) = Some (b,o) ->
+    Maps.PTree.get id (Genv.genv_symb ge) = Some (b,o) \/
+    (symbentry_id se = Some id /\ is_symbol_internal se = false).
+Proof.
+  unfold add_external_global. simpl. intros.
+  destr_in H. simpl in H. destr_in H.
+  rewrite Maps.PTree.gsspec in H.
+  destr_in H. subst. inv H. auto.
+Qed.
+
+Lemma genv_symb_add_external_globals:
+  forall t stbl ge id b o,
+    Maps.PTree.get id (Genv.genv_symb (add_external_globals t ge stbl)) = Some (b,o) ->
+    Maps.PTree.get id (Genv.genv_symb ge) = Some (b,o) \/
+    (exists se,
+        In se stbl /\
+        symbentry_id se = Some id /\
+        is_symbol_internal se = false).
+Proof.
+  induction stbl. simpl. auto.
+  simpl. intros.
+  eapply IHstbl in H.
+  destruct H.
+  - apply genv_symb_add_external_global in H. destruct H; auto.
+    right. eexists; split. left; eauto. destruct H. auto.
+  - destruct H as (se & IN & EQ & EXT).
+    right; exists se; repeat split; auto.
+Qed.
+
+Lemma fold_acc_symb_map_in_stbl:
+  forall (id : positive) (stbl : symbtable) t0 (b : block) (o : ptrofs),
+  Maps.PTree.get id (fold_right acc_symb_map t0 stbl) = Some (b, o) ->
+  (exists se : symbentry, In se stbl /\ symbentry_id se = Some id) \/
+  Maps.PTree.get id t0 = Some (b, o).
+Proof.
+  induction stbl; simpl; intros; eauto.
+  unfold acc_symb_map in H at 1.
+  destr_in H.
+  - destr_in H.
+    + rewrite Maps.PTree.gsspec in H. destr_in H.
+      inv H.
+      left; eexists; split; eauto. eapply IHstbl in H; eauto.
+      destruct H; eauto. decompose [ex and] H. eauto.
+    + eapply IHstbl in H; eauto.
+      destruct H; eauto. decompose [ex and] H. eauto.
+    + eapply IHstbl in H; eauto.
+      destruct H; eauto. decompose [ex and] H. eauto.
+  - eapply IHstbl in H; eauto.
+    destruct H; eauto. decompose [ex and] H. eauto.
+Qed.
+
+Lemma gen_symb_map_in_stbl:
+  forall id stbl b o,
+    Maps.PTree.get id (gen_symb_map stbl) = Some (b, o) ->
+    exists se, In se stbl /\ symbentry_id se = Some id.
+Proof.
+  unfold gen_symb_map.
+  intros.
+  edestruct fold_acc_symb_map_in_stbl; eauto.
+  rewrite Maps.PTree.gempty in H0. congruence.
+Qed.
+
+Lemma genv_symb_in_defs:
+  forall p id b o,
+    Maps.PTree.get id (Genv.genv_symb (RelocProgSemantics.globalenv p)) = Some (b,o) ->
+    (exists se,
+        In se (prog_symbtable p) /\
+        symbentry_id se = Some id (* /\ *)
+        (* symbentry_secindex se = secindex_normal i /\ *)
+        (* b = sec_index_to_block i /\ *)
+        (* o = Ptrofs.repr (symbentry_value se) *)
+    ).
+Proof.
+  unfold RelocProgSemantics.globalenv.
+  intros.
+  eapply genv_symb_add_external_globals in H.
+  destruct H.
+  simpl in H.
+  - eapply gen_symb_map_in_stbl; eauto.
+  - decompose [ex and] H; eauto.
+Qed.
+
+Lemma prog_symtable_same:
+  prog_symbtable prog = prog_symbtable tprog.
+Proof.
+  clear ge tge.
+  unfold match_prog, Reloctablesgen.transf_program in TRANSF.
+  monadInv TRANSF. reflexivity.
+Qed.
+
+Lemma symb_address_has_symtable_entry:
+  forall i b o,
+    RelocProgSemantics.Genv.find_symbol ge i = Some (b, o) ->
+    exists idx s,
+      SeqTable.SeqTable.get idx (prog_symbtable tprog) = Some s /\
+      symbentry_id s = Some i.
+Proof.
+  intros i b o FS.
+  unfold SeqTable.SeqTable.get.
+  rewrite <- prog_symtable_same.
+  unfold RelocProgSemantics.Genv.find_symbol in FS.
+  edestruct genv_symb_in_defs as (se & IN & ID); eauto.
+  destruct (In_nth_error _ _ IN).
+  exists (N.of_nat x); eexists.
+  rewrite Nnat.Nat2N.id. eauto.
+Qed.
+
+Lemma fold_acc_symb_index_map_acc:
+  forall stbl i t0 t1 n ofs ofs',
+    (* list_norepet (map symbentry_id stbl) -> *)
+    ~ In (Some i) (map symbentry_id stbl) ->
+    Maps.PTree.get i t0 = Some n ->
+    fold_left acc_symb_index_map stbl (ofs, t0) = (ofs', t1) ->
+  Maps.PTree.get i t1 = Some n.
+Proof.
+  induction stbl; simpl; intros i t0 t1 n ofs ofs' NR GET FL.
+  - inv FL. auto.
+  - destr_in FL; eauto.
+    eapply IHstbl. 3: eauto. intuition.
+    rewrite Maps.PTree.gso; auto. intuition congruence.
+Qed.
+
+Lemma fold_acc_symb_index_map_ok:
+  forall (stbl1 stbl stbl2 : list symbentry) (e : symbentry) (i : ident) ofs t0,
+  stbl = stbl1 ++ e :: stbl2 ->
+  symbentry_id e = Some i ->
+  list_norepet (filter (fun a => match a with None => false | _ => true end) (map symbentry_id stbl)) ->
+  exists n junk,
+    fold_left acc_symb_index_map stbl1 (ofs, t0) = (n, junk) /\
+    Maps.PTree.get i
+                   (let '(_, map) := fold_left acc_symb_index_map stbl (ofs, t0) in map) =
+    Some n.
+Proof.
+  induction stbl1; simpl; intros; eauto.
+  - (do 2 eexists); split; eauto. subst. simpl. destr. destr_in Heqp. inv H0.
+    erewrite fold_acc_symb_index_map_acc; eauto. simpl in H1.
+    rewrite Heqo in H1. inv H1.
+    intro IN; apply H2. rewrite filter_In. auto.
+    rewrite Maps.PTree.gss. auto.
+  - destruct stbl. inv H. inv H. simpl.
+    eapply IHstbl1. eauto. auto.
+    simpl in H1. destr_in H1. inv H1. auto.
+Qed.
+
+Lemma gen_symb_index_map_ok:
+  forall stbl stbl1 stbl2 e i,
+  stbl = stbl1 ++ e :: stbl2 ->
+  symbentry_id e = Some i ->
+  list_norepet (filter (fun a => match a with None => false | _ => true end) (map symbentry_id stbl)) ->
+  exists n junk,
+    fold_left acc_symb_index_map stbl1 (0%N, Maps.PTree.empty _) = (n, junk) /\
+    Maps.PTree.get i (gen_symb_index_map stbl) = Some n.
+Proof.
+  unfold gen_symb_index_map.
+  intros; eapply fold_acc_symb_index_map_ok; eauto.
+Qed.
+
+(* Axiom ge_tge_ok: *)
+(*   forall (i0: ident) (o: Z) (i1: ptrofs), *)
+(*     (* Genv.find_symbol tge RELOC_DATA i0 = Some (b, o) -> *) *)
+(*     Maps.ZTree.get o (Genv.genv_reloc_ofs_symb tge RELOC_DATA) = Some i0 -> *)
+(*     RelocProgSemantics.Genv.symbol_address ge i0 i1 = Genv.symbol_address tge RELOC_DATA o i1. *)
+
+Require Import Lia.
+
+Lemma fold_acc_sym_len:
+  forall stbl1 o t0 n junk,
+    fold_left acc_symb_index_map stbl1 (o, t0) = (n, junk) ->
+    n = N.add (N.of_nat (length stbl1)) o.
+Proof.
+  induction stbl1; intros; eauto.
+  simpl in H; inv H. auto.
+  simpl in H. eapply IHstbl1 in H. subst.
+  simpl length.
+  lia.
+Qed.
+
+Lemma nth_error_nodup:
+  forall {T U} (l: list T) n1 n2 x y (f: T -> option U),
+  nth_error l n1 = Some x ->
+  nth_error l n2 = Some y ->
+  list_norepet (filter (fun a => match a with None => false  | _ => true end)
+                       (map f l)) ->
+  f x <> None ->
+  f x = f y ->
+  n1 = n2.
+Proof.
+  induction l; simpl; intros; eauto.
+  rewrite nth_error_nil in H. easy.
+  destruct n1, n2; simpl in *; auto.
+  - inv H. exfalso. destr_in H1. destr_in Heqb. inv H1. apply H5.
+    rewrite filter_In. split; auto.
+    rewrite in_map_iff. exists y; split; auto.
+    eapply nth_error_in; eauto. destr_in Heqb.
+  - inv H0. exfalso. destr_in H1. destr_in Heqb. inv H1. apply H5.
+    rewrite filter_In. split; auto.
+    rewrite in_map_iff. exists x; split; auto.
+    eapply nth_error_in; eauto. destr_in Heqb.
+  - f_equal. eapply IHl; eauto.
+    destr_in H1. inv H1; auto.
+Qed.
+
+Lemma transl_init_data_ok_all_symbs_in_sim:
+  forall i0 i1 init sim rdata,
+    In (Init_addrof i0 i1) init ->
+    transl_init_data_list sim init = OK rdata ->
+    Maps.PTree.get i0 sim <> None.
+Proof.
+  unfold transl_init_data_list.
+  intros i0 i1 init sim rdata IN.
+  generalize (OK (0, @nil relocentry)).
+  revert init rdata IN.
+  induction init; simpl; intros; eauto.
+  monadInv H. destr_in EQ0. inv EQ0.
+  destruct IN.
+  - subst. simpl in EQ. destruct r. repeat destr_in EQ.
+    destr_in H0. destr_in H0. simpl in H0.
+    rewrite fold_acc_init_data_error in H0. congruence.
+    simpl in EQ.
+    rewrite fold_acc_init_data_error in EQ. congruence.
+  - eapply IHinit. auto. rewrite EQ. simpl. reflexivity.
+Qed.
+
+Lemma in_acc_symb_index_map_in_stbl:
+  forall (i0 : positive) (stbl : symbtable) o map o' map',
+    fold_left acc_symb_index_map stbl (o, map) = (o', map') ->
+    Maps.PTree.get i0 map' <> None ->
+    Maps.PTree.get i0 map <> None \/
+    exists s : symbentry, In s stbl /\ symbentry_id s = Some i0.
+Proof.
+  induction stbl; simpl; intros; eauto. inv H. auto.
+  eapply IHstbl in H.
+  destruct H. destr_in H.
+  rewrite Maps.PTree.gsspec in H. destr_in H. subst. right; eauto.
+  destruct H as (s & IN & ID); eauto. auto.
+Qed.
+
+Lemma in_sim_in_stbl:
+  forall i0 stbl,
+    Maps.PTree.get i0 (gen_symb_index_map stbl) <> None ->
+    exists s, In s stbl /\ symbentry_id s = Some i0.
+Proof.
+  unfold gen_symb_index_map. intros. destr_in H.
+  eapply in_acc_symb_index_map_in_stbl in H; eauto.
+  rewrite Maps.PTree.gempty in H. intuition congruence.
+Qed.
+
+Lemma in_stbl_in_gen_symb_map:
+  forall s i0 i stbl,
+    In s stbl ->
+    symbentry_id s = Some i0 ->
+    symbentry_secindex s = secindex_normal i ->
+    Maps.PTree.get i0 (gen_symb_map stbl) <> None.
+Proof.
+  unfold gen_symb_map.
+  intros s i0 i stbl.
+  generalize (Maps.PTree.empty (block * ptrofs)).
+  revert stbl.
+  induction stbl; simpl; intros; eauto.
+  destruct H.
+  - subst.
+    unfold acc_symb_map at 1. rewrite H0, H1.
+    rewrite Maps.PTree.gss. congruence.
+  - specialize (IHstbl t H H0 H1).
+    unfold acc_symb_map at 1.
+    destr. destr.
+    rewrite Maps.PTree.gsspec. destr.
+Qed.
+
+Lemma add_external_globals_acc:
+  forall stbl ge i0 extfuns,
+    Maps.PTree.get i0 (Genv.genv_symb ge) <> None ->
+    Maps.PTree.get i0 (Genv.genv_symb (add_external_globals extfuns ge stbl)) <> None.
+Proof.
+  induction stbl; simpl; intros; eauto.
+  apply IHstbl.
+  unfold add_external_global.
+  destr. simpl. destr.
+  rewrite Maps.PTree.gsspec. destr.
+Qed.
+
+Lemma in_stbl_external_in_genv_symb:
+  forall s i0 extfuns stbl ge,
+    In s stbl ->
+    symbentry_id s = Some i0 ->
+    is_symbol_internal s = false ->
+    Maps.PTree.get i0 (Genv.genv_symb (add_external_globals extfuns ge stbl)) <> None.
+Proof.
+  induction stbl; simpl; intros; eauto.
+  destruct H.
+  - subst.
+    apply add_external_globals_acc.
+    unfold add_external_global. rewrite H0. simpl.
+    rewrite H1.
+    rewrite Maps.PTree.gss. congruence.
+  - eauto.
+Qed.
+
+Lemma in_stbl_in_genv_symb:
+  forall s i0,
+    In s (prog_symbtable prog) ->
+    symbentry_id s = Some i0 ->
+    Maps.PTree.get i0 (Genv.genv_symb ge) <> None.
+Proof.
+  intros.
+  unfold ge. unfold RelocProgSemantics.globalenv.
+  destruct (is_symbol_internal s) eqn:INT.
+  - apply add_external_globals_acc. simpl.
+    unfold is_symbol_internal in INT. destr_in INT.
+    eapply in_stbl_in_gen_symb_map; eauto.
+  - eapply in_stbl_external_in_genv_symb; eauto.
+Qed.
+
+Lemma in_sim_find_symbol_not_none:
+  forall i0,
+    Maps.PTree.get i0 (gen_symb_index_map (prog_symbtable prog)) <> None ->
+    RelocProgSemantics.Genv.find_symbol ge i0 <> None.
+Proof.
+  unfold RelocProgSemantics.Genv.find_symbol.
+  intros.
+  edestruct in_sim_in_stbl as (s & IN & ID); eauto.
+  eapply in_stbl_in_genv_symb; eauto.
+Qed.
+
+Axiom norepet_symbentry_id:
+  list_norepet
+    (filter (fun a => match a with
+                      | Some _ => true
+                      | None => false
+                      end) symbentry_id ## (prog_symbtable tprog)).
+
+
+Lemma transl_init_data_norepet:
+  forall sim z0 a r,
+    transl_init_data sim z0 a = OK r ->
+    list_norepet reloc_offset ## r.
+Proof.
+  destruct a; simpl; intros; inv H; simpl ; try econstructor.
+  repeat destr_in H1. simpl. repeat constructor. easy.
+Qed.
+
+Lemma transl_init_data_range:
+  forall sim z0 a r,
+    transl_init_data sim z0 a = OK r ->
+    Forall (fun e => z0 <= reloc_offset e < z0 + init_data_size a) r.
+Proof.
+  destruct a; simpl; intros; inv H; simpl ; try econstructor.
+  repeat destr_in H1. constructor. 2: constructor.
+  simpl. destr; omega.
+Qed.
+
+Lemma norepet_fold_acc_init_data:
+  forall sim init z0 rdata0 z1 rdata1,
+    list_norepet reloc_offset ## rdata0 ->
+    Forall (fun e => reloc_offset e < z0) rdata0 ->
+    fold_left (acc_init_data sim) init (OK (z0, rdata0)) = OK (z1, rdata1) ->
+    list_norepet reloc_offset ## rdata1.
+Proof.
+  induction init; simpl; intros z0 rdata0 z1 rdata1 NR0 LT0 FL; eauto.
+  - inv FL; auto.
+  - destruct (transl_init_data sim z0 a) eqn:TID.
+    + simpl in *.
+      exploit IHinit. 3: eauto.
+      * rewrite map_app. rewrite list_norepet_app.
+        split; [|split]; auto.
+        eapply transl_init_data_norepet; eauto.
+        red. intros.
+        intro EQ; subst.
+        rewrite Forall_forall in LT0.
+        apply transl_init_data_range in TID.
+        rewrite Forall_forall in TID.
+        rewrite in_map_iff in H, H0.
+        decompose [ex and] H.
+        decompose [ex and] H0. subst.
+        specialize (LT0 _ H5).
+        specialize (TID _ H3).
+        omega.
+      * rewrite Forall_forall. intros x. rewrite in_app.
+        apply transl_init_data_range in TID.
+        rewrite Forall_forall in LT0, TID.
+        destruct 1. apply TID in H. omega.
+        apply LT0 in H. generalize (init_data_size_pos a). omega.
+      * auto.
+    + simpl in FL. rewrite fold_acc_init_data_error in FL. congruence.
+Qed.
+
+Lemma norepet_reloctables:
+  forall sim init rdata,
+    transl_init_data_list sim init = OK rdata ->
+    list_norepet reloc_offset ## rdata.
+Proof.
+  unfold transl_init_data_list. intros.
+  monadInv H. repeat destr_in EQ0.
+  eapply norepet_fold_acc_init_data; eauto. constructor.
+Qed.
+
+Lemma store_init_data_ok:
+  forall i m b o m' l1 l2 rtbl init,
+    let sim := gen_symb_index_map (prog_symbtable prog) in
+    init = l1 ++ i :: l2 ->
+    transl_init_data_list sim init = OK (reloctable_data (prog_reloctables tprog)) ->
+    fold_left (acc_init_data sim) l1 (OK (0, [])) = OK (o, rtbl) ->
+    RelocProgSemantics.store_init_data ge m b o i = Some m' ->
+    store_init_data tge m b o i = Some m'.
+Proof.
+  intros i m b o m' l1 l2 rtbl init sim SPLIT TIDL FOLD SID.
+  unfold RelocProgSemantics.store_init_data, store_init_data in *.
+  destr_in SID.
+  unfold RelocProgSemantics.Genv.symbol_address in SID.
+  unfold Genv.symbol_address.
+  destr_in SID. destr_in SID.
+  edestruct symb_address_has_symtable_entry as (idx & s & GET & ID). eauto.
+  edestruct in_split as (stbl1 & stbl2 & EQ). eapply nth_error_In.
+  unfold SeqTable.SeqTable.get in GET. apply GET.
+  edestruct gen_symb_index_map_ok as (n & junk & FL & SYMGET). eauto. eauto.
+  eapply norepet_symbentry_id.
+  edestruct transl_init_data_list_ok as (e & ofs & rtbl' & INreloc & FL2 & ROFS & TYP & RSYM & RADD).
+  3: eauto. eauto. eauto.
+  rewrite <- prog_symtable_same. fold sim. apply TIDL. eauto.
+  exploit fold_acc_sym_len. apply FL. intro Neq.
+  exploit (@nth_error_nodup). exact GET.
+  rewrite EQ. rewrite nth_error_app2. instantiate (2:= length stbl1).
+  rewrite Nat.sub_diag. reflexivity. omega.
+  eapply norepet_symbentry_id. congruence. reflexivity. intro idxEQ.
+  erewrite symb_address_2. eauto. 3: eauto. eauto.
+  eapply norepet_reloctables. eauto.
+  eauto.  3: eauto.
+  rewrite RSYM. rewrite Neq. rewrite <- idxEQ. rewrite Nnat.N2Nat.id. lia.
+  rewrite ROFS.
+  revert FL2 FOLD. rewrite <- prog_symtable_same. fold sim.
+  congruence.
+  eapply in_sim_find_symbol_not_none in Heqo0. easy.
+  eapply transl_init_data_ok_all_symbs_in_sim. 2: eauto. rewrite SPLIT.
+  apply in_app. right. left. reflexivity.
+Qed.
+
+Lemma transl_init_data_list_inv:
+  forall sim init dreloc a,
+    transl_init_data_list sim init = OK dreloc ->
+    In a init ->
+    exists o ri, transl_init_data sim o a = OK ri.
+Proof.
+  unfold transl_init_data_list.
+  intros sim init dreloc a.
+  generalize (OK (0, @nil relocentry)).
+  revert init dreloc a.
+  induction init; simpl; intros; eauto. easy.
+  destruct H0; subst; eauto.
+  unfold acc_init_data at 2 in H.
+  monadInv H. repeat destr_in EQ0.
+  destruct r; simpl in *; eauto.
+  destruct p; simpl in *; eauto.
+  destruct (transl_init_data sim z0 a0) eqn:?; simpl in *.
+  eauto.
+  rewrite fold_acc_init_data_error in EQ; congruence.
+  rewrite fold_acc_init_data_error in EQ; congruence.
+Qed.
+
+
+Lemma store_init_data_list_ok:
+  forall i m b o m' init l1 rtbl,
+    let sim := gen_symb_index_map (prog_symbtable prog) in
+    init = l1 ++ i ->
+    transl_init_data_list sim init = OK (reloctable_data (prog_reloctables tprog)) ->
+    fold_left (acc_init_data sim) l1 (OK (0, [])) = OK (o, rtbl) ->
+    RelocProgSemantics.store_init_data_list ge m b o i = Some m' ->
+    store_init_data_list tge m b o i = Some m'.
+Proof.
+  induction i; simpl; intros; eauto.
+  destr_in H2.
+  erewrite store_init_data_ok.
+  3: eauto. 2: eauto. 2: eauto. 2: eauto.
+  edestruct (transl_init_data_list_inv) as (oo & ri & TID). apply H0. subst.
+  rewrite in_app; right; left; eauto.
+  rewrite transl_init_data_translate in TID.
+  monadInv TID.
+  eapply IHi. 2: eauto. instantiate (1:=l1 ++ a :: nil). rewrite <- app_assoc. simpl. auto.
+  rewrite fold_left_app. rewrite H1. simpl.
+  rewrite transl_init_data_translate, EQ. simpl.
+  f_equal.  auto.
+Qed.
+
+Lemma prog_sectable_eq:
+  exists init c c',
+    prog_sectable prog = [sec_null; sec_data init; sec_text c] /\
+    transl_code' c = OK c' /\
+    prog_sectable tprog = [sec_null; sec_data init; sec_text c'] /\
+    transl_init_data_list (gen_symb_index_map (prog_symbtable prog)) init =
+    OK (reloctable_data (prog_reloctables tprog)).
+Proof.
+  unfold match_prog, transf_program in TRANSF.
+  monadInv TRANSF. simpl in *.
+  exploit transl_sectable_ok. eauto.
+  intros (c & l & CODE & DATA & TCODE & TDATA).
+  unfold transl_sectable' in EQ1. repeat destr_in EQ1. monadInv H0. simpl.
+  (do 3 eexists). split. eauto. split. eauto. split. eauto.
+  vm_compute in DATA. inv DATA. auto.
+Qed.
+
+Lemma alloc_data_section_ok:
+  forall m0 m,
+    RelocProgSemantics.alloc_data_section ge (prog_sectable prog) m0 = Some m ->
+    alloc_data_section tge (prog_sectable tprog) m0 = Some m.
+Proof.
+  intros m0 m ADS.
+  unfold RelocProgSemantics.alloc_data_section, alloc_data_section in *.
+  repeat destr_in ADS.
+  destruct (prog_sectable_eq) as (init' & c & c' & PS1 & TC & PS2 & TIDL).
+  rewrite PS2. simpl.
+  rewrite PS1 in Heqo. vm_compute in Heqo. inv Heqo.
+  simpl in *.
+  rewrite Heqp. rewrite Heqo0.
+  erewrite store_init_data_list_ok; eauto. rewrite app_nil_l. auto. reflexivity.
+Qed.
+
+Lemma code_size_app:
+  forall l1 l2,
+    code_size (l1 ++ l2) = code_size l1 + code_size l2.
+Proof.
+  induction l1; simpl; intros; eauto. rewrite IHl1. omega.
+Qed.
+
+Lemma code_size_rev:
+  forall l,
+    code_size l = code_size(rev l).
+Proof.
+  induction l; simpl; intros; eauto.
+  rewrite code_size_app. rewrite IHl. simpl. omega.
+Qed.
+
+Lemma id_eliminate_size:
+  forall i1 i2,
+    id_eliminate i1 = OK i2 ->
+    instr_size i1 = instr_size i2.
+Proof.
+  intros i1 i2 IE.
+  unfold id_eliminate in IE.
+  repeat destr_in IE; simpl; auto.
+Qed.
+
+Lemma fold_acc_id_eliminate_error:
+  forall c e,
+    fold_left acc_id_eliminate c (Error e) = Error e.
+Proof.
+  induction c; simpl; intros; eauto.
+Qed.
+
+Lemma transl_code_fold_size:
+  forall c r x,
+    fold_left acc_id_eliminate c (OK r) = OK x ->
+    code_size (rev x) = code_size (r) + code_size c.
+Proof.
+  induction c; simpl; intros; eauto. inv H. rewrite <- code_size_rev. omega.
+  destruct (id_eliminate a) eqn:?.
+  simpl in H.
+  apply IHc in H. rewrite H. simpl.
+  apply id_eliminate_size in Heqr0; rewrite Heqr0. omega.
+  simpl in H. rewrite fold_acc_id_eliminate_error in H; congruence.
+Qed.
+
+Lemma transl_code_size:
+  forall c c',
+    transl_code' c = OK c' ->
+    code_size c' = code_size c.
+Proof.
+  unfold transl_code'.
+  intros c c' FL.
+  monadInv FL.
+  erewrite transl_code_fold_size; eauto. simpl. omega.
+Qed.
+
+Lemma alloc_code_section_ok:
+  forall m0 m,
+    RelocProgSemantics.alloc_code_section (prog_sectable prog) m0 = Some m ->
+    alloc_code_section (prog_sectable tprog) m0 = Some m.
+Proof.
+  intros m0 m ACS.
+  unfold RelocProgSemantics.alloc_code_section, alloc_code_section in *.
+  repeat destr_in ACS.
+  destruct (prog_sectable_eq) as (init' & c & c' & PS1 & TC & PS2 & TIDL).
+  rewrite PS2. simpl.
+  rewrite PS1 in Heqo. vm_compute in Heqo. inv Heqo.
+  erewrite transl_code_size; eauto.
+  simpl in *.
+  rewrite Heqp. auto.
+Qed.
+
+Lemma alloc_external_symbols_ok:
+  forall m1,
+    alloc_external_symbols m1 (prog_symbtable tprog) =
+    RelocProgSemantics.alloc_external_symbols m1 (prog_symbtable prog).
+Proof.
+  rewrite prog_symtable_same.
+  generalize (prog_symbtable tprog).
+  induction s; simpl; intros; eauto.
+Qed.
+
+Lemma init_mem_ok:
+  forall m,
+    RelocProgSemantics.init_mem prog = Some m ->
+    init_mem tprog = Some m.
+Proof.
+  intros m IM.
+  unfold RelocProgSemantics.init_mem, init_mem in *.
+  repeat destr_in IM.
+  erewrite alloc_data_section_ok; eauto.
+  erewrite alloc_code_section_ok; eauto.
+  apply alloc_external_symbols_ok.
+Qed.
+
+Lemma main_preserved:
+  prog_main prog = prog_main tprog.
+Proof.
+  unfold match_prog, transf_program in TRANSF.
+  monadInv TRANSF. reflexivity.
+Qed.
+
+
+Lemma main_ok:
+  RelocProgSemantics.Genv.symbol_address ge (prog_main prog) Ptrofs.zero =
+  RelocProgSemantics.Genv.symbol_address (Genv.genv_genv tge) (prog_main tprog) Ptrofs.zero.
+Proof.
+  rewrite main_preserved.
+  unfold RelocProgSemantics.Genv.symbol_address.
+  unfold tge.
+  unfold ge.
+  unfold globalenv. simpl.
+  unfold RelocProgSemantics.Genv.find_symbol.
+  rewrite genv_symb_ok. auto.
+Qed.
+
+Lemma defs_preserved:
+  prog_defs prog = prog_defs tprog.
+Proof.
+  unfold match_prog, transf_program in TRANSF.
+  monadInv TRANSF. reflexivity.
+Qed.
+
+Lemma ext_funs_add_external_global:
+  forall efs s ge1 ge2,
+    Genv.genv_ext_funs ge1 = Genv.genv_ext_funs ge2 ->
+    Genv.genv_next ge1 = Genv.genv_next ge2 ->
+    Genv.genv_ext_funs (add_external_global efs ge1 s) =
+    Genv.genv_ext_funs (add_external_global efs ge2 s) /\
+    Genv.genv_next (add_external_global efs ge1 s) =
+    Genv.genv_next (add_external_global efs ge2 s).
+Proof.
+  unfold add_external_global. intros.
+  repeat destr; simpl; intuition congruence.
+Qed.
+
+Lemma ext_funs_add_external_globals:
+  forall efs stbl ge1 ge2,
+    Genv.genv_ext_funs ge1 = Genv.genv_ext_funs ge2 ->
+    Genv.genv_next ge1 = Genv.genv_next ge2 ->
+    Genv.genv_ext_funs (add_external_globals efs ge1 stbl) =
+    Genv.genv_ext_funs (add_external_globals efs ge2 stbl) /\
+    Genv.genv_next (add_external_globals efs ge1 stbl) =
+    Genv.genv_next (add_external_globals efs ge2 stbl).
+Proof.
+  induction stbl; simpl; intros; eauto.
+  exploit ext_funs_add_external_global; eauto. intros (A & B).
+  apply IHstbl; eauto.
+Qed.
+
+Lemma find_ext_funct_ok:
+  forall v,
+  RelocProgSemantics.Genv.find_ext_funct ge v =
+  Genv.find_ext_funct tge v.
+Proof.
+  unfold Genv.find_ext_funct, RelocProgSemantics.Genv.find_ext_funct.
+  intros. destr.
+  unfold tge, globalenv. simpl. unfold ge.
+  unfold RelocProgSemantics.globalenv.
+  f_equal.
+  rewrite defs_preserved.
+  rewrite prog_symtable_same.
+  apply ext_funs_add_external_globals; reflexivity.
+Qed.
+
+
+Lemma instrs_add_external_global:
+  forall efs s ge1,
+    Genv.genv_instrs (add_external_global efs ge1 s) = Genv.genv_instrs ge1.
+Proof.
+  unfold add_external_global. intros.
+  repeat destr.
+Qed.
+
+Lemma instrs_add_external_globals:
+  forall efs stbl ge1,
+    Genv.genv_instrs (add_external_globals efs ge1 stbl) =
+    Genv.genv_instrs ge1.
+Proof.
+  induction stbl; simpl; intros; eauto.
+  erewrite IHstbl. erewrite instrs_add_external_global; eauto.
+Qed.
+
+Lemma fold_acc_id_eliminate_app:
+  forall c c0,
+    fold_left acc_id_eliminate c (OK c0) =
+    bind (fold_left acc_id_eliminate c (OK [])) (fun c1 => OK (c1 ++ c0)).
+Proof.
+  induction c; simpl; intros; eauto.
+  destruct (id_eliminate a) eqn:?.
+  simpl.
+  rewrite (IHc (i::c0)).
+  rewrite (IHc ([i])).
+  destruct (fold_left acc_id_eliminate c (OK [])) eqn:?.
+  simpl. rewrite <- app_assoc. simpl. reflexivity.
+  simpl. auto.
+  simpl. rewrite ! fold_acc_id_eliminate_error. reflexivity.
+Qed.
+
+Lemma gen_instr_map_ok:
+  forall c ofs0 map0 map0' ofs1 ofs1' map1 map1' c1
+         (REC:
+            forall iofs i,
+              map0 iofs = Some i ->
+              exists i', map0' iofs = Some i' /\ id_eliminate i = OK i'
+         )
+         iofs i
+         (GenInstrMap: fold_left acc_instr_map c (ofs0, map0) = (ofs1, map1))
+         (SrcInstr: map1 iofs = Some i)
+         (TranslCode: fold_left acc_id_eliminate c (OK []) = OK (c1))
+         (TgtGenInstrMap: fold_left acc_instr_map (rev c1) (ofs0, map0') = (ofs1', map1')),
+  ofs1 = ofs1' /\ exists i', map1' iofs = Some i' /\ id_eliminate i = OK i'.
+Proof.
+  induction c; simpl; intros; eauto.
+  - inv TranslCode. inv GenInstrMap.
+    simpl in TgtGenInstrMap. inv TgtGenInstrMap.
+    (* apply (f_equal (@length _)) in H0. rewrite app_length in H0. *)
+    (* assert (length c1 = O) by omega. destruct c1. simpl in H1. inv H1; auto. *)
+    (* simpl in H. omega. *)
+    eauto.
+  - destruct (id_eliminate a) eqn:?.
+    + simpl in TranslCode.
+      rewrite fold_acc_id_eliminate_app in TranslCode. monadInv TranslCode.
+      subst.
+      rewrite rev_app_distr in TgtGenInstrMap. simpl in TgtGenInstrMap.
+      eapply IHc. 2: eauto. 2: eauto. 2: eauto.
+      2: erewrite id_eliminate_size; eauto.
+      simpl.
+      intros. destr_in H. inv H. eauto. eauto.
+    + simpl in TranslCode.
+      rewrite fold_acc_id_eliminate_error in TranslCode. congruence.
+Qed.
+
+
+Lemma find_instr_ok:
+  forall v i,
+  RelocProgSemantics.Genv.find_instr ge v = Some i ->
+  exists i',
+    Genv.find_instr tge v = Some i' /\
+    id_eliminate i = OK i'.
+Proof.
+  unfold Genv.find_instr.
+  unfold tge.
+  unfold globalenv. simpl.
+  unfold RelocProgSemantics.Genv.find_instr.
+  intros. destr.
+  unfold ge in H.
+  unfold RelocProgSemantics.globalenv in *.
+  rewrite instrs_add_external_globals in *. simpl in *.
+  destruct (prog_sectable_eq) as (init & c & c' & PS1 & TC & PS2 & TIDL).
+  rewrite PS1, PS2 in *.
+  simpl in *.
+  unfold gen_instr_map, transl_code' in *.
+  destr_in H. monadInv TC. destr.
+  intros.
+  eapply gen_instr_map_ok. 3: apply H. 2: eauto. 3: eauto. 2: eauto.
+  simpl. easy.
+Qed.
+
+
+Definition addrmode_reloc_id (a:addrmode) : res ident :=
+  let '(Addrmode base ofs const) := a in
+  match const with
+  | inr (id, _) => OK id
+  | _ => Error (msg "addrmode_reloc_id")
+  end.
+
+Definition instr_reloc_id (i:instruction) : res ident :=
+  match i with
+  | Pmov_rs _ id => OK id
+  | Pcall (inr id) _ => OK id
+  | Pjmp (inr id) _ => OK id
+  | Pleal _ a
+  | Pmovl_rm _ a
+  | Pmovl_mr a _
+  | Pmov_rm_a _ a
+  | Pmov_mr_a a _ => addrmode_reloc_id a
+  | _ => Error (msg "Calculation of relocation offset failed: Either there is no possible relocation location or the instruction is not supported yet by relocation")
+  end.
+
+
+Lemma exec_instr_ok:
+  forall i rs m rs' m' i' bpc opc
+         (PC: rs PC = Vptr bpc opc)
+         (SYMBS: forall idofs id ofs,
+             instr_reloc_id i = OK id ->
+             id_reloc_offset (Ptrofs.unsigned opc) i = Some idofs ->
+             Genv.symbol_address tge RELOC_CODE idofs ofs =
+             RelocProgSemantics.Genv.symbol_address ge id ofs)
+         (EI: RelocProgSemantics.exec_instr ge i rs m = Next rs' m')
+         (ELIM : id_eliminate i = OK i'),
+    exec_instr tge i' rs m = Next rs' m'.
+Proof.
+  intros.
+  destruct i; simpl in *; inv EI; inv ELIM; simpl; eauto;
+    try (unfold exec_instr, get_pc_offset; rewrite PC; auto; fail).
+  - unfold exec_instr. unfold get_pc_offset; rewrite PC; auto.
+    simpl in *.
+    erewrite SYMBS. 2: eauto. 2: reflexivity. auto.
+  -
+    assert (i' =  Pmovl_rm rd match a with
+                              | Addrmode rb ss (inl _) => a
+                              | Addrmode rb ss (inr (_, ptrofs)) =>
+                                Addrmode rb ss (inr (1%positive, ptrofs))
+                              end).
+    repeat destr_in H1; inv H1. clear H1. subst.
+    unfold exec_instr. unfold get_pc_offset.
+    rewrite PC. unfold id_reloc_offset. Opaque Z.add. simpl.
+    unfold exec_load. unfold RelocProgSemantics.exec_load.
+    match goal with
+    | |-
+      match Mem.loadv _ _ ?v1 with _ => _ end =
+      match Mem.loadv _ _ ?v2 with _ => _ end =>
+      let x := fresh in
+      assert (x: v1 = v2); [|rewrite x; auto]
+    end.
+    {
+      destr. destr. destr.
+      unfold eval_addrmode, RelocProgSemantics.eval_addrmode.
+      destr.
+      unfold eval_addrmode64, RelocProgSemantics.eval_addrmode64.
+      f_equal. f_equal. apply  SYMBS. reflexivity. reflexivity.
+      unfold eval_addrmode32, RelocProgSemantics.eval_addrmode32.
+      f_equal. f_equal. apply  SYMBS. reflexivity. reflexivity.
+    }
+    repeat destr.
+  - admit.                      (* to check... *)
+  - assert (i' =  Pmovl_mr match a with
+                           | Addrmode rb ss (inl _) => a
+                           | Addrmode rb ss (inr (_, ptrofs)) =>
+                             Addrmode rb ss (inr (1%positive, ptrofs))
+                           end rs0).
+    repeat destr_in H1; inv H1. clear H1. subst.
+    unfold exec_instr. unfold get_pc_offset.
+    rewrite PC. unfold id_reloc_offset. Opaque Z.add. simpl.
+    unfold exec_store. unfold RelocProgSemantics.exec_store.
+    match goal with
+    | |-
+      match Mem.storev _ _ ?v1 _ with _ => _ end =
+      match Mem.storev _ _ ?v2 _ with _ => _ end =>
+      let x := fresh in
+      assert (x: v1 = v2); [|rewrite x; auto]
+    end.
+    {
+      destr. destr. destr.
+      unfold eval_addrmode, RelocProgSemantics.eval_addrmode.
+      destr.
+      unfold eval_addrmode64, RelocProgSemantics.eval_addrmode64.
+      f_equal. f_equal. apply  SYMBS. reflexivity. reflexivity.
+      unfold eval_addrmode32, RelocProgSemantics.eval_addrmode32.
+      f_equal. f_equal. apply  SYMBS. reflexivity. reflexivity.
+    }
+    repeat destr.
+  - admit.
+  - unfold exec_instr. unfold get_pc_offset.
+    rewrite PC. unfold id_reloc_offset. Opaque Z.add. simpl.
+    unfold exec_load. unfold RelocProgSemantics.exec_load.
+    match goal with
+    | |-
+      match Mem.loadv _ _ ?v1 with _ => _ end =
+      match Mem.loadv _ _ ?v2 with _ => _ end =>
+      let x := fresh in
+      assert (x: v1 = v2); [|rewrite x; auto]
+    end.
+    {
+      unfold eval_addrmode, RelocProgSemantics.eval_addrmode.
+      destr.
+      unfold eval_addrmode64, RelocProgSemantics.eval_addrmode64.
+      destr.
+      f_equal. f_equal. repeat destr.
+      unfold RelocProgSemantics.Genv.symbol_address.
+      apply  SYMBS. reflexivity. reflexivity.
+      unfold eval_addrmode32, RelocProgSemantics.eval_addrmode32.
+      f_equal. f_equal. apply  SYMBS. reflexivity. reflexivity.
+    }
+    repeat destr.
+
+
+
+Qed.
+
+
 Lemma transf_program_correct:
   forall rs, forward_simulation (RelocProgSemantics.semantics prog rs)
                                 (RelocProgSemantics1.semantics tprog rs).
@@ -44,10 +1339,29 @@ Proof.
     rewrite ! genv_senv_add_external_globals. simpl. auto.
   - intros s1 IS. eexists; split; eauto.
     unfold semantics. simpl. inv IS. simpl in *.
-    econstructor.
+    exploit init_mem_ok; eauto. intro IM.
+    econstructor. eauto.
+    inv H0.
+    unfold rs0, ge0. fold ge. rewrite main_ok.
+    econstructor; eauto.
+  - intros. subst. simpl in *.
+    inv H0. constructor; auto.
+  - simpl.
+    intros. subst. inv H.
+    edestruct find_instr_ok as (i' & FI & ELIM); eauto.
+    exploit exec_step_internal. eauto.
+    erewrite <- find_ext_funct_ok; eauto.
+    eauto.
 
-
-Admitted.
+    (* exec_step_internal
+     : forall (ge : Genv.t) (b : block) (ofs : ptrofs) (i : instruction) (rs : preg -> val) 
+         (m : mem) (rs' : regset) (m' : mem),
+       rs PC = Vptr b ofs ->
+       Genv.find_ext_funct ge (Vptr b ofs) = None ->
+       Genv.find_instr ge (Vptr b ofs) = Some i ->
+       exec_instr ge i rs m = Next rs' m' -> step ge (State rs m) E0 (State rs' m')
+ *)
+Qed.
 
 End PRESERVATION.
 
